src/SerialFacts.v
@@ -1,32 +1,12 @@
 Require Import Bool List String Peano_dec.
 Require Import Common ListSupport FMap.
-Require Import Syntax Semantics SemFacts StepDet StepSeq Serial.
+Require Import Syntax Semantics SemFacts StepDet Serial.
 
 Set Implicit Arguments.
 
-Lemma transactional_cons_inv:
-  forall sys a ll,
-    Transactional sys (a :: ll) ->
-    Transactional sys ll.
-Proof.
-  unfold Transactional; intros.
-  destruct H as [ptid [pmin [pmouts [? ?]]]].
-  inv H0.
-  do 3 eexists; split; eauto.
-Qed.
-
-Corollary transactional_ocons_inv:
-  forall sys oa ll,
-    Transactional sys (oa ::> ll) ->
-    Transactional sys ll.
-Proof.
-  destruct oa as [a|]; simpl; intros; auto.
-  eauto using transactional_cons_inv.
-Qed.
-
 Lemma atomic_nil_in:
-  forall tid min mouts,
-    Atomic tid min nil mouts ->
+  forall sys tid min mouts,
+    Atomic sys tid min nil mouts ->
     forall msg,
       In msg mouts ->
       msg = min.
@@ -36,20 +16,11 @@ Proof.
   reflexivity.
 Qed.
 
-Lemma step_det_seq_in:
-  forall sys st1 msg st2,
-    step_det sys st1 (IlblIn msg) st2 ->
-    step_seq sys st1 (IlblIn msg) st2.
-Proof.
-  intros; inv H.
-  constructor; auto.
-Qed.
-
 Lemma steps_det_atomic_outs_ts:
-  forall tid min ll mouts,
-    Atomic tid min ll mouts ->
-    forall sys st1 st2,
-      steps step_det sys st1 ll st2 ->
+  forall sys tid min ll mouts,
+    Atomic sys tid min ll mouts ->
+    forall st1 st2,
+      steps_det sys st1 ll st2 ->
       Forall (fun tmsg => tmsg_tid tmsg = Some tid) mouts.
 Proof.
   induction 1; simpl; intros.
@@ -57,16 +28,16 @@ Proof.
   - inv H1; apply Forall_app.
     + apply Forall_remove; eauto.
     + apply step_det_outs_tid in H7; dest; auto.
-      specialize (IHAtomic _ _ _ H5).
+      specialize (IHAtomic _ _ H5).
       eapply Forall_forall in IHAtomic; [|eassumption].
       rewrite <-IHAtomic; auto.
 Qed.
 
 Lemma steps_det_atomic_outs_fwd_tid:
-  forall tid min ll mouts,
-    Atomic tid min ll mouts ->
-    forall sys st1 st2,
-      steps step_det sys st1 ll st2 ->
+  forall sys tid min ll mouts,
+    Atomic sys tid min ll mouts ->
+    forall st1 st2,
+      steps_det sys st1 ll st2 ->
       Forall (fun l => match l with
                        | IlblOuts (Some hdl) _ => tmsg_tid hdl = Some tid
                        | _ => False
@@ -79,92 +50,20 @@ Proof.
   eapply Forall_forall in H; eauto.
 Qed.
 
-Lemma transactional_steps_seq:
-  forall sys ll,
-    Transactional sys ll ->
-    forall st1 st2,
-      steps step_det sys st1 ll st2 ->
-      steps step_seq sys st1 ll st2.
-Proof.
-  induction ll as [|l ll]; simpl; intros; subst;
-    [inv H0; constructor|].
-
-  specialize (IHll (transactional_cons_inv H)).
-
-  destruct H as [tid [trin [trouts [? ?]]]].
-  pose proof (steps_det_atomic_outs_fwd_tid H1 H0).
-
-  inv H0.
-  specialize (IHll _ _ H6).
-  econstructor; eauto.
-
-  inv H2.
-  destruct l; [intuition idtac|].
-  destruct mhdl; [|intuition idtac].
-
-  destruct ll.
-  - inv H1; inv H11; inv H6.
-    Common.dest_in.
-    inv H8.
-    + econstructor; eauto.
-    + exfalso; simpl in H9; eauto using internal_external_false.
-  - inv H1; inv H11; inv H5.
-    inv H8.
-    + exfalso.
-      inv IHll.
-      apply step_seq_outs_tid in H22; simpl in H22; dest.
-      simpl in H4; inv H4.
-      rewrite H0 in H2; inv H2.
-      intuition.
-    + assert (ts = mts); subst.
-      { inv IHll.
-        apply step_seq_outs_tid in H22; simpl in H22; dest.
-        rewrite H14 in H4; inv H4.
-        rewrite H0 in H2; inv H2.
-        reflexivity.
-      }
-      econstructor; eauto.
-Qed.
-
-Lemma sequential_steps:
-  forall sys ll,
-    Sequential sys ll ->
-    forall st,
-      steps step_det sys (getStateInit sys) ll st ->
-      steps step_seq sys (getStateInit sys) ll st.
-Proof.
-  induction 1; simpl; intros; subst.
-  - inv H; constructor.
-  - inv H1.
-    econstructor; eauto.
-    apply step_det_seq_in; auto.
-  - eapply steps_split in H1; [|reflexivity].
-    destruct H1 as [sti ?]; dest.
-    apply steps_append with (st2:= sti); auto.
-    auto using transactional_steps_seq.
-Qed.
-
-Theorem serializable_step_seq:
-  forall sys ll st,
-    steps step_det sys (getStateInit sys) ll st ->
-    Serializable sys step_det ll ->
-    Behavior step_seq sys (behaviorOf sys ll).
-Proof.
-  unfold Serializable; intros.
-  destruct H0 as [sll [sst [? [? ?]]]].
-  pose proof (sequential_steps H1 H0) as Hseq.
-  eapply Behv; eauto.
-Qed.
-
-Theorem sequential_step_seq:
+Theorem serializable_seqSteps_refines:
   forall sys,
-    SerializableSys sys step_det ->
-    step_det # step_seq |-- sys ⊑[id] sys.
+    SerializableSys sys ->
+    steps_det # seqSteps |-- sys ⊑[id] sys.
 Proof.
   unfold SerializableSys, Refines; intros.
-  inv H0; rename ll0 into ill. (* ill: the interleaving label sequence *)
+  inv H0; rename ll0 into ill.
   specialize (H _ _ H1).
-  rewrite map_id.
-  eauto using serializable_step_seq.
+
+  unfold Serializable in H.
+  destruct H as [sll [sst [? ?]]].
+
+  rewrite H0.
+  econstructor; eauto.
+  apply map_id.
 Qed.
 
