src/TrsSim.v
@@ -1,0 +1,88 @@
+Require Import Bool List String Peano_dec.
+Require Import Common FMap Syntax Semantics StepDet SemFacts.
+Require Import Simulation Serial.
+
+Require Import Omega.
+
+Set Implicit Arguments.
+
+Section TrsSim.
+  Variables (sim: TState -> TState -> Prop)
+            (p: Label -> Label).
+
+  Local Infix "≈" := sim (at level 30).
+
+  Variables (impl spec: System).
+
+  Definition TrsSimulates :=
+    forall ist1 sst1,
+      ist1 ≈ sst1 ->
+      forall ihst ist2,
+        trsSteps impl ist1 ihst ist2 ->
+        exists sst2 shst,
+          map p (behaviorOf impl ihst) = behaviorOf spec shst /\
+          steps_det spec sst1 shst sst2 /\
+          ist2 ≈ sst2.
+
+  Hypothesis (Hsim: TrsSimulates).
+
+  Lemma trs_simulation_steps:
+    forall ist1 sst1,
+      ist1 ≈ sst1 ->
+      forall trss ihst ist2,
+        Forall (Transactional impl) trss ->
+        ihst = concat trss ->
+        steps_det impl ist1 ihst ist2 ->
+        exists sst2 shst,
+          map p (behaviorOf impl ihst) = behaviorOf spec shst /\
+          steps_det spec sst1 shst sst2 /\
+          ist2 ≈ sst2.
+  Proof.
+    induction trss as [|trs trss]; simpl; intros; subst.
+    - inv H2; exists sst1, nil; repeat split.
+      + constructor.
+      + assumption.
+    - inv H0.
+      eapply steps_split in H2; [|reflexivity].
+      destruct H2 as [sti [? ?]].
+      specialize (IHtrss _ _ H5 eq_refl H0).
+      destruct IHtrss as [isst [ishst [? [? ?]]]].
+      pose proof (Hsim H6 (conj H1 H4)).
+      destruct H7 as [sst2 [shst [? [? ?]]]].
+      do 2 eexists; repeat split.
+      + instantiate (1:= _ ++ _).
+        do 2 rewrite behaviorOf_app.
+        rewrite map_app.
+        rewrite H2, H7; reflexivity.
+      + eapply steps_append; eauto.
+      + assumption.
+  Qed.
+
+  Corollary simulation_seqSteps:
+    forall ist1 sst1,
+      ist1 ≈ sst1 ->
+      forall ihst ist2,
+        seqSteps impl ist1 ihst ist2 ->
+        exists sst2 shst,
+          map p (behaviorOf impl ihst) = behaviorOf spec shst /\
+          steps_det spec sst1 shst sst2 /\
+          ist2 ≈ sst2.
+  Proof.
+    unfold seqSteps, Sequential; intros; dest; subst.
+    eapply trs_simulation_steps; eauto.
+  Qed.
+
+  Hypothesis (Hsimi: sim (getStateInit impl) (getStateInit spec)).
+
+  Theorem sequential_simulation_implies_refinement:
+    seqSteps # steps_det |-- impl ⊑[p] spec.
+  Proof.
+    unfold Simulates, Refines; intros.
+    inv H.
+    eapply simulation_seqSteps in H0; [|exact Hsimi].
+    destruct H0 as [sst2 [shst [? [? ?]]]].
+    econstructor; eauto.
+  Qed.
+
+End TrsSim.
+  
